translator/ml_translator_testScript.sml
@@ -198,10 +198,29 @@ val map_again_def = Define `map_again f [] = []
 
 val inc_list_def = Define `inc_list xs = map_again (\x. x + SUC 0) xs`;
 
-val _ = reset_translation ();
-
 val r = abs_translate map_again_def;
 val r = abs_translate inc_list_def;
 val r = concretise [``map_again``, ``inc_list``];
+
+(* check EqualityType proves for some modestly complex datatypes *)
+
+val _ = Datatype `a_type = AT_Nil | AT_Rec (a_type list) ((a_type # num) list)`;
+val _ = Datatype `a_b_type = ABT_Nil
+  | ABT_Rec (bool list) ((a_b_type # num) list)`;
+val _ = Datatype.Hol_datatype `a_c_type = ACT_Nil
+  | ACT_One of 'a | ACT_Two of 'b | ACT_Rec of (a_c_type # num) list`;
+
+val r = register_type ``:a_type``;
+val r = register_type ``:a_b_type``;
+val r = register_type ``:('a, 'b) a_c_type``;
+
+val a_inv = get_type_inv ``:a_type``;
+val a_b_inv = get_type_inv ``:a_b_type``;
+val a_c_inv_num = get_type_inv ``:(num, num) a_c_type``;
+
+val EqTyp_test_lemmas = Q.store_thm ("EqTyp_test_lemmas",
+  `EqualityType (^a_inv) /\ EqualityType (^a_b_inv)
+    /\ EqualityType (^a_c_inv_num)`,
+  fs (eq_lemmas ()));
 
 val _ = export_theory();
